Update to version TCS 2026.

finddefs.ml
@@ -1,0 +1,70 @@
+(* ========================================================================= *)
+(* Find ML definitions in HOL Light sources.                                 *)
+(* (Very crude and simplistic, yet sufficiently useful.)                     *)
+(*                                                                           *)
+(* (c) Copyright, Antonella Bilotta, Marco Maggesi, Cosimo Perini Brogi 2026 *)
+(* ========================================================================= *)
+
+(* ------------------------------------------------------------------------- *)
+(* Compilation:                                                              *)
+(*   ocamlc -I +str str.cma -o finddefs finddefs.ml                          *)
+(* Usage:                                                                    *)
+(*   find *.ml -type f -print0 | xargs -n1 -0 finddefs > DEFS.tex            *)
+(* ------------------------------------------------------------------------- *)
+
+let let_re = Str.regexp "^let[ \t]+\\([A-Za-z0-9_']+\\)"
+let end_re = Str.regexp ".*;;[ \t\r]*$"
+
+let extract_id line =
+  if Str.string_match let_re line 0 then
+    Some (Str.matched_group 1 line)
+  else
+    None
+
+let find_defs file =
+  let ic = open_in file in
+
+  let rec loop line_no current acc =
+    match input_line ic with
+    | exception End_of_file ->
+        close_in ic;
+        List.rev acc
+
+    | line ->
+        let line_no = line_no + 1 in
+
+        let current, acc =
+          match current with
+          | None ->
+              begin match extract_id line with
+              | None ->
+                  None, acc
+
+              | Some id ->
+                  if Str.string_match end_re line 0 then
+                    None, (id, line_no, line_no) :: acc
+                  else
+                    Some (id, line_no), acc
+              end
+
+          | Some (id, start_line) ->
+              if Str.string_match end_re line 0 then
+                None, (id, start_line, line_no) :: acc
+              else
+                current, acc
+        in
+
+        loop line_no current acc
+  in
+  loop 0 None []
+
+let () =
+  if Array.length Sys.argv <> 2 then begin
+    Printf.eprintf "Uso: %s file.ml\n" Sys.argv.(0);
+    exit 1
+  end;
+
+  let path = Sys.argv.(1) in
+  find_defs path
+  |> List.iter (fun (id, i, j) ->
+       Printf.printf "\\srccode{%s}{%s}{%d}{%d}\n" id path i j)
