conjlist.ml
@@ -5,7 +5,7 @@
 (* (c) Copyright, Antonella Bilotta, Marco Maggesi,                          *)
 (*                Cosimo Perini Brogi, Leonardo Quartini 2024.               *)
 (* (c) Copyright, Antonella Bilotta, Marco Maggesi,                          *)
-(*                Cosimo Perini Brogi 2025-26.                               *)
+(*                Cosimo Perini Brogi 2025-2026.                             *)
 (* ========================================================================= *)
 
 needs "HOLMS/calculus.ml";;
