gen_decid_after.ml
@@ -2,7 +2,7 @@
 (* Some additional theorem-tactics.                                          *)
 (*                                                                           *)
 (* (c) Copyright, Antonella Bilotta, Marco Maggesi,                          *)
-(*                Cosimo Perini Brogi 2026.                                  *)
+(*                Cosimo Perini Brogi 2025-2026.                             *)
 (* ========================================================================= *)
 
 let HOLDS_NNFC_UNFOLD_CONV : conv =
@@ -52,6 +52,7 @@ let HOLDS_SIMP_THEN : thm_tactical =
 let SATURATE_STRIP_THEN : thm_tactical =
   FIRST_TCL [CONJUNCTS_THEN; DISJ_CASES_THEN; IMP_RES_THEN'; HOLDS_SIMP_THEN];;
 
+(* TODO: Fattorizzare con TRIVIAL_ASSUME_LITERAL_THEN. *)
 let rec SATURATE_TAC thl th =
   (REPEAT_TCL SATURATE_STRIP_THEN)
   (fun th ->
