s4_completeness.ml
@@ -1,7 +1,7 @@
 (* Proof of the consistency and modal completeness of S4.                     *)
 (*                                                                           *)
 (* (c) Copyright, Antonella Bilotta, Marco Maggesi,                          *)
-(*                Cosimo Perini Brogi 2025.                                  *)
+(*                Cosimo Perini Brogi 2025-2026.                             *)
 (* ========================================================================= *)
 
 needs "HOLMS/gen_completeness.ml";;
@@ -272,7 +272,7 @@ e (CLAIM_TAC "consistent_X"
         (CONS (Not q)
               (FLATMAP (\x. match x with Box c -> [c; Box c] | _ -> []) w))`);;
   e (REMOVE_THEN "contra" MP_TAC);;
-  e (REWRITE_TAC[CONSISTENT; CONTRAPOS_THM]);;
+  e (REWRITE_TAC[CONSISTENT_ALT; CONTRAPOS_THM]);;
   e (INTRO_TAC "incons" THEN MATCH_MP_TAC MAXIMAL_CONSISTENT_LEMMA);;
   e (MAP_EVERY EXISTS_TAC
        [`S4_AX`;
@@ -307,7 +307,7 @@ e (CLAIM_TAC "consistent_X"
     e (MESON_TAC[MLK_axiom_not;MLK_iff_imp2]);;
    e (MESON_TAC[MLK_imp_refl_th]);;
   e (POP_ASSUM MATCH_MP_TAC);;
-  e (HYP_TAC "incons" (REWRITE_RULE[CONSISTENT]));;
+  e (HYP_TAC "incons" (REWRITE_RULE[CONSISTENT_ALT]));;
   e (HYP_TAC "incons" (ONCE_REWRITE_RULE[CONJLIST]));;
   e (POP_ASSUM MP_TAC);;
   e (COND_CASES_TAC);;
